decrypt goes through modulo a three local assumes (plainlen <>0ul, which should be removed; and a local regression in CMA wrapper that arose from the overnight reindexing of mac logs with nonces; and showing that fresh nonces remain unused after decrypt)

examples/low-level/crypto/Crypto.AEAD.BufferUtils.fst
@@ -8,43 +8,66 @@ module HS = FStar.HyperStack
 
 type buffer = Buffer.buffer UInt8.t
 
-let prf_mac_modifies (c:bool) (r:rid) h0 h1 = 
-  if c then h0 == h1 else modifies_transitively (as_set [r]) h0 h1
+abstract let prf_mac_modifies (prf_region:rid) (mac_region:rid) h0 h1 = 
+  h0 == h1  \/
+  (HS.modifies_transitively (as_set [prf_region]) h0 h1       /\ //only touched the prf's region (and its children)
+   HS.modifies_ref mac_region TSet.empty h0 h1)                 //in the mac region, didn't touch any existing ref
 
-let dexor_modifies (c:bool) (r:rid) (b:buffer) (h0:mem) (h1:mem) =
+let intro_prf_mac_modifies (prf_region:rid) (mac_region:rid) (h0:mem) (h1:mem)
+  : Lemma (requires (h0 == h1  \/
+		     (HS.modifies_transitively (as_set [prf_region]) h0 h1 /\ 
+		      HS.modifies_ref mac_region TSet.empty h0 h1)))
+          (ensures (prf_mac_modifies prf_region mac_region h0 h1))
+  = ()
+
+let dexor_modifies (c:bool) (prf_region:rid) (plain:buffer) (h0:mem) (h1:mem) =
    if c
-   then Buffer.modifies_1 b h0 h1
-   else (HS.modifies_transitively (as_set [r; frameOf b]) h0 h1 /\
-	 Buffer.modifies_buf_1 (frameOf b) b h0 h1)
+   then Buffer.modifies_1 plain h0 h1
+   else (HS.modifies (as_set [prf_region; frameOf plain]) h0 h1 /\
+	 Buffer.modifies_buf_1 (frameOf plain) plain h0 h1)
 
-let decrypt_modifies (c:bool) (r:rid) (b:buffer) (h0:mem) (h1:mem) = 
-  if c
-  then Buffer.modifies_1 b h0 h1
-  else  HS.modifies_transitively (as_set [r; frameOf b]) h0 h1 /\
-        Buffer.modifies_buf_1 (frameOf b) b h0 h1
+let decrypt_modifies (prf_region:rid) (mac_region:rid)
+		     (plain:buffer) (h0:mem) (h1:mem) : Type0 =  //TODO: strange, seem to need the Type0 annotation otherwise code below fails
+  HS.modifies_transitively (as_set [prf_region; frameOf plain]) h0 h1 /\ 
+  Buffer.modifies_buf_1 (Buffer.frameOf plain) plain h0 h1 /\
+  HS.modifies_ref mac_region TSet.empty h0 h1
 
-val chain_modification: cond:bool -> log_region:rid -> b:buffer -> 
-			(h_init:mem) -> (h0:mem) ->(h1:mem)-> (h2:mem) -> (h3:mem) -> (h4:mem) ->
-     Lemma (requires
-	      Buffer.live h_init b /\
-	      log_region `is_in` h_init.h /\
-	      is_eternal_region log_region /\
-	      is_eternal_region (frameOf b) /\
-	      HH.disjoint (frameOf b) log_region /\
-	      HS.fresh_frame h_init h0 /\
-	      prf_mac_modifies cond log_region h0 h1 /\
-	      Buffer.modifies_0 h1 h2 /\
-	      Buffer.modifies_0 h2 h3 /\
-	      (h3 == h4 \/ dexor_modifies cond log_region b h3 h4))
+let accumulate_modifies_nothing h0 h1 = 
+  let open HS in
+  modifies_one h0.tip h0 h1
+  /\ Buffer.modifies_buf_0 h0.tip h0 h1
+  /\ h0.tip=h1.tip
+
+val chain_modification: #a:Type -> 
+			acc:FStar.Buffer.buffer a ->
+			cond:bool -> 
+			prf_region:rid -> 
+			mac_region:rid -> 
+			plain:buffer -> //plain
+			h_init:mem -> 
+			h0:mem -> //after push
+			h1:mem -> //after prf_mac
+			h2:mem -> //after accumulate
+			h3:mem -> //after verify
+			h4:mem -> //after dexor
+     Lemma (requires 
+	      Buffer.live h_init plain /\
+	      prf_region `is_in` h_init.h /\
+	      mac_region `is_in` h_init.h /\
+	      is_eternal_region prf_region /\
+	      is_eternal_region (frameOf plain) /\
+	      prf_region `HH.includes` mac_region /\
+	      prf_region <> mac_region /\
+	      HH.disjoint (frameOf plain) prf_region /\
+	      HS.fresh_frame h_init h0 /\                        //push
+	      prf_mac_modifies prf_region mac_region h0 h1 /\    //prf_mac
+	      accumulate_modifies_nothing h1 h2 /\               //accumulate
+	      Buffer.frameOf acc = h2.tip /\
+	      Buffer.modifies_1 acc h2 h3 /\                      //verify
+	      (h3 == h4 \/ dexor_modifies cond prf_region plain h3 h4)) //maybe dexor
 	    (ensures (HS.poppable h4 /\
-		      decrypt_modifies cond log_region b h_init (HS.pop h4)))
+		      decrypt_modifies prf_region mac_region plain h_init (HS.pop h4)))
 #reset-options "--initial_fuel 0 --initial_ifuel 0 --max_fuel 0 --max_ifuel 0 --z3rlimit 100"
-let chain_modification cond log_region b h_init h0 h1 h2 h3 h4 =
-    Buffer.lemma_reveal_modifies_0 h1 h2;
-    Buffer.lemma_reveal_modifies_0 h2 h3;
-    FStar.Classical.move_requires (Buffer.lemma_reveal_modifies_1 b h3) h4;
-    if cond then begin
-      assert (HS.modifies (as_set [h0.tip]) h0 h3);
-      Buffer.lemma_intro_modifies_1 b h_init (HS.pop h4)
-    end
-    else ()
+let chain_modification #a acc cond prf_region mac_region plain h_init h0 h1 h2 h3 h4 =
+    Buffer.lemma_reveal_modifies_1 acc h2 h3;
+    FStar.Classical.move_requires (Buffer.lemma_reveal_modifies_1 plain h3) h4
